simplify bitmaps

lib/Lib.Bitmap.fst
@@ -1,363 +1,80 @@
 module Lib.Bitmap
 
-open Lib.IntTypes
 open Lib.Sliceable
 
 module IT = Lib.IntTypes
 
 #set-options "--fuel 0 --ifuel 0"
 
-private inline_for_extraction noextract val aux (t:inttype{unsigned t}) (l:secrecy_level) : (xN:sig (bits t){xN.t == int_t t l})
-private inline_for_extraction noextract
-let aux t l =
-{ t = int_t t l
-; v = (fun x i -> FStar.UInt.nth #(bits t) (v x) i)
-; mk = (fun f -> mk_int (UInt.from_vec #(bits t) (FStar.Seq.init (bits t) f)))
+inline_for_extraction noextract val uN (t:IT.inttype{IT.unsigned t}) (l:IT.secrecy_level) : (xN:sig (IT.bits t){xN.t == IT.int_t t l})
+inline_for_extraction noextract
+let uN t l =
+{ t = IT.int_t t l
+; v = (fun x i -> FStar.UInt.nth #(IT.bits t) (IT.v x) i)
+; mk = (fun f -> IT.mk_int (UInt.from_vec #(IT.bits t) (FStar.Seq.init (IT.bits t) f)))
 ; mk_def = (fun f i -> ())
-; ones_ = Lib.IntTypes.ones t l
-; zeros_ = Lib.IntTypes.zeros t l
-; and_ = logand
-; xor_ = logxor
-; or_ = logor
-; not_ = lognot
-; zeros_spec = (fun i -> UInt.zero_nth_lemma #(bits t) i)
-; ones_spec = (fun i -> UInt.ones_nth_lemma #(bits t) i)
-; and_spec = (fun x y i -> logand_spec x y)
-; xor_spec = (fun x y i -> logxor_spec x y)
-; or_spec = (fun x y i -> logor_spec x y)
-; not_spec = (fun x i -> lognot_spec x)
+; ones_ = IT.ones t l
+; zeros_ = IT.zeros t l
+; and_ = IT.logand
+; xor_ = IT.logxor
+; or_ = IT.logor
+; not_ = IT.lognot
+; zeros_spec = (fun i -> UInt.zero_nth_lemma #(IT.bits t) i)
+; ones_spec = (fun i -> UInt.ones_nth_lemma #(IT.bits t) i)
+; and_spec = (fun x y i -> IT.logand_spec x y)
+; xor_spec = (fun x y i -> IT.logxor_spec x y)
+; or_spec = (fun x y i -> IT.logor_spec x y)
+; not_spec = (fun x i -> IT.lognot_spec x)
 }
 
 inline_for_extraction noextract
-val bitmap (t:inttype{unsigned t}) (l:secrecy_level) (n:nat) : Type0
-inline_for_extraction noextract
-let rec bitmap t l n = if n <= bits t then int_t t l else int_t t l * bitmap t l (n-bits t)
-
-inline_for_extraction noextract
-val uN (t:inttype{unsigned t}) (l:secrecy_level) (n:nat{n<=bits t}): (xN:sig n{xN.t == bitmap t l n})
-#push-options "--fuel 1"
-inline_for_extraction noextract
-let uN t l n =
-  if n = bits t then
-    aux t l
-  else
-    xN_rest (aux t l) n
-#pop-options
-
-inline_for_extraction noextract
 val uN_eq
-  (#t1 #t2:(t:inttype{unsigned t})) (#l:secrecy_level)
-  (#n:nat{n<=bits t1 /\ n<=bits t2})
-  (x:(uN t1 l n).t) (y:(uN t2 l n).t) : Type0
+  (#t1 #t2:(t:IT.inttype{IT.unsigned t})) (#l:IT.secrecy_level)
+  (x:(uN t1 l).t) (y:(uN t2 l).t) : Type0
 inline_for_extraction noextract
 let uN_eq x y = forall i. (_).v x i == (_).v y i
 
 inline_for_extraction noextract
-val lemma0 (n:nat) (m:nat{n<=m}) (a:FStar.UInt.uint_t n) (i:nat{i<n}) :
-  Lemma (FStar.UInt.size a m /\ FStar.UInt.nth #m a i == FStar.UInt.nth #n a i)
-inline_for_extraction noextract
-let rec lemma0 n m a i =
-  if n=0 then (
-    ()
-  ) else (
-    admit ()
-  )
-
-inline_for_extraction noextract
-val uN_cast (#t1 t2:(t:inttype{unsigned t})) (#l:secrecy_level) (#n:nat{n<=bits t1 /\ n<=bits t2}) (x:(uN t1 l n).t) :
-  Pure (uN t2 l n).t (requires True) (ensures fun y -> uN_eq y x)
-inline_for_extraction noextract
-let uN_cast #t1 t2 #l #n x =
-  let n1 = bits t1 in
-  let n2 = bits t2 in
-  let a : int_t t1 l = x in
-  let b : int_t t2 l = cast t2 l a in
-  let y : (uN t2 l n).t = b in
-  assert(forall (i:nat{i<n}). (_).v y i == FStar.UInt.nth #n2 (v a % pow2 n2) i);
-  let aux (i:nat{i<n}) : Lemma (FStar.UInt.nth #n2 (v a % pow2 n2) i == FStar.UInt.nth #n1 (v a) i) =
-    if n = 0 then ( ()
-    ) else if n2<n1 then (
-      lemma0 n2 n1 (v a % pow2 n2) i;
-      lemma0 n2 n1 (pow2 n2 - 1) i
-    ) else (
-      lemma0 n1 n2 (v a) i
-    )
-  in
-  FStar.Classical.forall_intro aux;
-  assert(forall (i:nat{i<n}). FStar.UInt.nth #n2 (v a % pow2 n2) i == FStar.UInt.nth #n1 (v a) i);
-  y
-
-inline_for_extraction noextract
-val uN_expend (#t:(t:inttype{unsigned t})) (#l:secrecy_level) (#n:nat{n<=bits t}) (m:nat{n<=m /\ m<=bits t}) (x:(uN t l n).t) :
-  Pure (uN t l m).t (requires True) (ensures fun y -> forall (i:nat{i<n}). (_).v y i == (_).v x i)
-inline_for_extraction noextract
-let uN_expend m x = x
-
-inline_for_extraction noextract
-val uN_reduce (#t:(t:inttype{unsigned t})) (#l:secrecy_level) (#n:nat{n<=bits t}) (m:nat{m<=n}) (x:(uN t l n).t) :
-  Pure (uN t l m).t (requires True) (ensures fun y -> forall (i:nat{i<m}). (_).v y i == (_).v x i)
-inline_for_extraction noextract
-let uN_reduce m x = x
-
-inline_for_extraction noextract
 val uN_shift_left
-  (#t:inttype{unsigned t}) (#l:secrecy_level) (#n:nat{n<=bits t})
-  (x:(uN t l n).t) (k:nat{k<bits t}) :
-  Pure (uN t l n).t
+  (#t:IT.inttype{IT.unsigned t}) (#l:IT.secrecy_level)
+  (x:(uN t l).t) (k:nat{k<IT.bits t}) :
+  Pure (uN t l).t
     (requires True)
-    (ensures fun y -> forall (i:nat{i<n-k}). (_).v y i == (_).v x (i+k))
+    (ensures fun y -> forall (i:nat{i<IT.bits t-k}). (_).v y i == (_).v x (i+k))
 inline_for_extraction noextract
-let uN_shift_left #t #l #n x k =
-  let y : (uN t l n).t = shift_left #t #l x (size k) in
-  let aux (i:nat{i<n-k}) : Lemma ((_).v y i == (_).v x (i+k)) =
-    if n=0 then
+let uN_shift_left #t #l x k =
+  let y : (uN t l).t = IT.shift_left #t #l x (IT.size k) in
+  let aux (i:nat{i<IT.bits t-k}) : Lemma ((_).v y i == (_).v x (i+k)) =
+    if IT.bits t=0 then
       ()
     else
-      FStar.UInt.shift_left_lemma_2 #(bits t) (v #t #l x) k i
+      FStar.UInt.shift_left_lemma_2 #(IT.bits t) (IT.v #t #l x) k i
   in
   FStar.Classical.forall_intro aux;
   y
 
 inline_for_extraction noextract
 val uN_shift_right
-  (#t:inttype{unsigned t}) (#l:secrecy_level) (#n:nat{n<=bits t})
-  (x:(uN t l n).t) (k:nat{k<bits t}) :
-  Pure (uN t l n).t
+  (#t:IT.inttype{IT.unsigned t}) (#l:IT.secrecy_level) (#n:nat{n<=IT.bits t})
+  (x:(uN t l).t) (k:nat{k<IT.bits t}) :
+  Pure (uN t l).t
     (requires True)
     (ensures fun y -> forall (i:nat{i<n}). (_).v y i == (if i<k then false else (_).v x (i-k)))
 inline_for_extraction noextract
 let uN_shift_right #t #l #n x k =
-  let y : (uN t l n).t = shift_right #t #l x (size k) in
+  let y : (uN t l).t = IT.shift_right #t #l x (IT.size k) in
   let aux (i:nat{i<n}) : Lemma ((_).v y i == (if i<k then false else (_).v x (i-k))) =
     if n=0 then (
       ()
     ) else if i<k then (
-      FStar.UInt.shift_right_lemma_1 #(bits t) (v #t #l x) k i
+      FStar.UInt.shift_right_lemma_1 #(IT.bits t) (IT.v #t #l x) k i
     ) else (
-      FStar.UInt.shift_right_lemma_2 #(bits t) (v #t #l x) k i
+      FStar.UInt.shift_right_lemma_2 #(IT.bits t) (IT.v #t #l x) k i
     )
   in
   FStar.Classical.forall_intro aux;
   y
 
 inline_for_extraction noextract
-val uN_concat
-  (#t1:inttype{unsigned t1}) (#l:secrecy_level)
-  (t2:inttype{unsigned t2})
-  (#n:nat{n<=bits t1 /\ n+n<=bits t2})
-  (x y:(uN t1 l n).t) :
-  Pure (uN t2 l (n+n)).t
-    (requires True)
-    (ensures fun z -> forall (i:nat{i<n+n}). (_).v z i == (if i<n then (_).v x i else (_).v y (i-n)))
-#push-options "--z3rlimit 100"
-inline_for_extraction noextract
-let uN_concat #t1 #l t2 #n x y =
-  let mask : (uN t2 l (n+n)).t = (_).not_ (uN_shift_right (_).ones_ n) in
-  assert(forall (i:nat{i<n+n}). (_).v mask i == (if i<n then true else false));
-  let x' : (uN t2 l (n+n)).t = uN_expend (n+n) (uN_cast t2 x) in
-  assert (forall (i:nat{i<n+n}). (_).v x' i == (if i<n then (_).v x i else (_).v x' i));
-  let x' : (uN t2 l (n+n)).t = (_).and_ x' mask in
-  assert(forall (i:nat{i<n+n}). (_).v x' i == (if i<n then (_).v x i else false));
-  let y' : (uN t2 l (n+n)).t = uN_expend (n+n) (uN_cast t2 y) in
-  assert(forall (i:nat{i<n+n}). (_).v y' i == (if i<n then (_).v y i else (_).v y' i));
-  let y' : (uN t2 l (n+n)).t = uN_shift_right #t2 #l #(n+n) y' n in
-  assert(forall (i:nat{i<n+n}). (_).v y' i == (if i<n then false else (_).v y (i-n)));
-  (_).or_ x' y'
-#pop-options
-
-inline_for_extraction noextract
-val uN_split
-  (#t1:inttype{unsigned t1}) (#l:secrecy_level)
-  (t2:inttype{unsigned t2})
-  (#n:nat{n+n<=bits t1 /\ n<=bits t2})
-  (x:(uN t1 l (n+n)).t) :
-  Pure ((uN t2 l n).t * (uN t2 l n).t)
-    (requires True)
-    (ensures fun (y, z) -> forall (i:nat{i<n+n}). (_).v (uN_concat t1 y z) i == (_).v x i)
-#push-options "--z3rlimit 100"
-inline_for_extraction noextract
-let uN_split #t1 #l t2 #n x =
-  let y : (uN t2 l n).t = uN_cast t2 (uN_reduce n x) in
-  assert(forall (i:nat{i<n}). (_).v y i == (_).v x i);
-  let z : (uN t2 l n).t = uN_cast t2 (uN_reduce n (uN_shift_left x n)) in
-  assert(forall (i:nat{i<n}). (_).v z i == (_).v x (i+n));
-  FStar.Classical.forall_intro (fun (i:nat{i<n+n}) ->
-    ( if i<n then (
-        assert((_).v (uN_concat t1 y z) i == (_).v y i)
-      ) else (
-        assert((i-n)+n == i);
-        assert((_).v (uN_concat t1 y z) i == (_).v z (i-n));
-        assert((_).v z (i-n) == (_).v x ((i-n)+n))
-      )
-    ) <: Lemma ((_).v (uN_concat t1 y z) i == (_).v x i)
-  ) <: Lemma (forall (i:nat{i<n+n}). (_).v (uN_concat t1 y z) i == (_).v x i);
-  (y, z)
-
-inline_for_extraction noextract
-let uNxM (t:inttype{unsigned t}) (l:secrecy_level) (n:nat{n<=bits t}) (m:IT.size_nat) : Type0 =
-  xNxM (uN t l n) m
-
-inline_for_extraction noextract
-val uNxM_h_concat
-  (#t1:inttype{unsigned t1}) (#l:secrecy_level)
-  (t2:inttype{unsigned t2})
-  (#n:nat{n<=bits t1 /\ n+n<=bits t2}) (#m:IT.size_nat)
-  (x y:uNxM t1 l n m) :
-  Pure (uNxM t2 l (n+n) m)
-    (requires True)
-    (ensures fun z -> forall (i:nat{i<n+n}) (j:nat{j<m}).
-      (_).v (index z j) i == (if i<n then (_).v (index x j) i else (_).v (index y j) (i-n))
-    )
-inline_for_extraction noextract
-let uNxM_h_concat t2 x y =
-  xNxM_mk _ _ (fun i -> uN_concat t2 (index x i) (index y i))
-
-inline_for_extraction noextract
-val uNxM_h_split
-  (#t1:inttype{unsigned t1}) (#l:secrecy_level)
-  (t2:inttype{unsigned t2})
-  (#n:nat{n+n<=bits t1 /\ n<=bits t2}) (#m:IT.size_nat)
-  (x:uNxM t1 l (n+n) m) :
-  Pure (uNxM t2 l n m * uNxM t2 l n m)
-    (requires True)
-    (ensures fun (y, z) -> forall (i:nat{i<n+n}) (j:nat{j<m}).
-      (_).v (index (uNxM_h_concat t1 y z) j) i == (_).v (index x j) i
-    )
-#push-options "--z3rlimit 100"
-inline_for_extraction noextract
-let uNxM_h_split #t1 #l t2 #n #m x =
-  let aux1 (a, b) = a in
-  let aux2 (a, b) = b in
-  let y : uNxM t2 l n m = xNxM_mk _ _ (fun j -> aux1 (uN_split t2 (index x j))) in
-  let z : uNxM t2 l n m = xNxM_mk _ _ (fun j -> aux2 (uN_split t2 (index x j))) in
-  FStar.Classical.forall_intro_2 (fun (i:nat{i<n+n}) (j:nat{j<m}) ->
-    ( let a = aux1 (uN_split t2 (index x j)) in
-      let b = aux2 (uN_split t2 (index x j)) in
-      assert(uN_split t2 (index x j) == (a, b))
-    ) <: Lemma ((_).v (index (uNxM_h_concat t1 y z) j) i == (_).v (index x j) i)
-  );
-  (y, z)
-#pop-options
-
-//val uNxM_v_concat
-//  (#t:inttype{unsigned t}) (#l:secrecy_level)
-//  (#n:IT.size_nat{n<=bits t}) (#m:nat)
-//  (x y:uNxM t l n m) :
-//  Pure (uNxM t l n (m+m))
-//    (requires True)
-//    (ensures fun z -> forall (i:nat{i<n}) (j:nat{j<m+m}).
-//      (_).v (index z j) i == (if j<m then (_).v (index x j) i else (_).v (index y (j-m)) i)
-//    )
-//let uNxM_v_concat #t #l #n #m x y =
-//  xNxM_mk _ _ (fun i -> if i<m then index x i else index y (i-m))
-//
-//val uNxM_v_split
-//  (#t:inttype{unsigned t}) (#l:secrecy_level)
-//  (#n:nat{n<=bits t}) (#m:nat)
-//  (x:uNxM t l n (m+m)) :
-//  Pure (uNxM t l n m * uNxM t l n m)
-//    (requires True)
-//    (ensures fun (y, z) -> forall (i:nat{i<n}) (j:nat{j<m+m}).
-//      (_).v (index (uNxM_v_concat y z) j) i == (_).v (index x j) i
-//    )
-//#push-options "--z3rlimit 100"
-//let uNxM_v_split #t #l #n #m x =
-//  let y = xNxM_mk _ _ (fun j -> index x j) in
-//  let z = xNxM_mk _ _ (fun j -> index x (j+m)) in
-//  FStar.Classical.forall_intro_2 (fun i j ->
-//    ( if j<m then (
-//        assert ((_).v (index (uNxM_v_concat y z) j) i == (_).v (index y j) i)
-//      ) else (
-//        assert ((_).v (index (uNxM_v_concat y z) j) i == (_).v (index z (j-m)) i);
-//        assert (index z (j-m) == index x ((j-m)+m));
-//        assert (index x ((j-m)+m) == index x j)
-//      )
-//    ) <:Lemma ((_).v (index (uNxM_v_concat y z) j) i == (_).v (index x j) i)
-//  );
-//  (y, z)
-//#pop-options
-
-//let foo (n:nat) = (t:inttype{unsigned t /\ n<=bits t})
-//
-//type transposable : (n:nat -> foo n -> m:nat -> foo m -> Type0) =
-//| Tr1 : t1:foo 1 -> t2:foo 1 -> transposable 1 t1 1 t2
-//| TrH : n:nat -> m:nat -> #t1:foo n -> #t2:foo m -> t3:foo (n+n) -> transposable n t1 m t2 -> transposable (n+n) t3 m t2
-//| TrV : n:nat -> m:nat -> #t1:foo n -> #t2:foo m -> t3:foo (m+m) -> transposable n t1 m t2 -> transposable n t1 (m+m) t3
-//
-//val transpose
-//  (#n #m:nat) (#t1:foo n) (#l:secrecy_level) (#t2:foo m)
-//  (pr:transposable n t1 m t2)
-//  (x:uNxM t1 l n m) :
-//  Pure (uNxM t2 l m n)
-//    (requires True)
-//    (ensures fun y -> forall (i:nat{i<n}) (j:nat{j<m}). (_).v (index y i) j == (_).v (index x j) i)
-//    (decreases pr)
-//#push-options "--ifuel 1 --z3rlimit 100"
-//let rec transpose #n #m #t1 #l #t2 pr x =
-//  match pr with
-//  | Tr1 _ _ -> xNxM_mk _ _ (fun 0 -> uN_cast t2 (index x 0))
-//  | TrH n m #t3 #t2 t1 pr' ->
-//    let (y, z) : (uNxM t3 l n m * uNxM t3 l n m) = uNxM_h_split t3 (x <: uNxM t1 l (n+n) m) in
-//    let y' : uNxM t2 l m n = transpose pr' y in
-//    let z' : uNxM t2 l m n = transpose pr' z in
-//    let w : uNxM t2 l m (n+n) = uNxM_v_concat y' z' in
-//    w
-//  | TrV n m #t1 #t3 t2 pr' ->
-//    let (y, z) : (uNxM t1 l n m * uNxM t1 l n m) = uNxM_v_split (x <: uNxM t1 l n (m+m)) in
-//    let y' : uNxM t3 l m n = transpose pr' y in
-//    let z' : uNxM t3 l m n = transpose pr' z in
-//    let w : uNxM t2 l (m+m) n = uNxM_h_concat t2 y' z' in
-//    w
-//#pop-options
-//
-//val transpose_inv (#n #m:nat) (#t1:foo n) (#t2:foo m) (pr:transposable n t1 m t2) :
-//  Pure (transposable m t2 n t1) (requires True) (ensures fun _ -> True) (decreases pr)
-//#push-options "--ifuel 1"
-//let rec transpose_inv pr = match pr with
-//| Tr1 t1 t2 -> Tr1 t2 t1
-//| TrH n m #t1 #t2 t3 pr -> TrV m n #t2 #t1 t3 (transpose_inv pr)
-//| TrV n m #t1 #t2 t3 pr -> TrH m n #t2 #t1 t3 (transpose_inv pr)
-//#pop-options
-//
-//val transpose_8_8 : transposable 8 U8 8 U8
-//let transpose_8_8 =
-//    TrH 4 8 U8
-//  ( TrV 4 4 U8
-//  ( TrH 2 4 U8
-//  ( TrV 2 2 U8
-//  ( TrH 1 2 U8
-//  ( TrV 1 1 U8
-//  ( Tr1 U8 U8
-//  ))))))
-//
-//val transpose_8_16 : transposable 8 U8 16 U16
-//let transpose_8_16 = TrV 8 8 U16 transpose_8_8
-//
-//val transpose_8_32 : transposable 8 U8 32 U32
-//let transpose_8_32 = TrV 8 16 U32 transpose_8_16
-//
-//val transpose_8_64 : transposable 8 U8 64 U64
-//let transpose_8_64 = TrV 8 32 U64 transpose_8_32
-//
-//val transpose_64_8 : transposable 64 U64 8 U8
-//let transpose_64_8 = transpose_inv transpose_8_64
-//
-//val line_transpose (#n #m:nat) (#t1:foo n) (#t2:foo m) (#l:secrecy_level) (x:uNxM t1 l n m) (i:nat{i<n})
-//  (pr:transposable n t1 m t2) :
-//    Lemma (line i (transpose pr x) == column i x)
-//  [SMTPat (line i (transpose pr x))]
-//let line_transpose x i pr = xNxM_eq_intro (line i (transpose pr x)) (column i x)
-//
-//val column_transpose (#n #m:nat) (#t1:foo n) (#t2:foo m) (#l:secrecy_level) (x:uNxM t1 l n m) (j:nat{j<m})
-//  (pr:transposable n t1 m t2) :
-//    Lemma (column j (transpose pr x) == line j x)
-//  [SMTPat (column j (transpose pr x))]
-//let column_transpose x j pr = xNxM_eq_intro (column j (transpose pr x)) (line j x)
-//
-//val transpose_transpose
-//  (#n #m:nat)
-//  (#t1:foo n) (#t2:foo m) (#t3:foo n) (#l:secrecy_level)
-//  (x:uNxM t1 l n m) (j:nat{j<m})
-//  (pr1:transposable n t1 m t2) (pr2:transposable m t2 n t3) :
-//    Lemma (line j (transpose pr2 (transpose pr1 x)) == line j x)
-//let transpose_transpose x j pr1 pr2 = ()
+let uNxM (t:IT.inttype{IT.unsigned t}) (l:IT.secrecy_level) (m:IT.size_nat) : Type0 =
+  xNxM (uN t l) m
